more veil-specific meta theory

LoL/MProp/NonDetT.lean
@@ -31,30 +31,54 @@ private lemma iInf_pi {α} {τ : α -> Type u} (p : (a : α) -> τ a -> l) [inst
       simp }
     intro i; apply iInf_le_of_le (i a); simp
 
+open Classical in
+private lemma iSup_pi {α} {τ : α -> Type u} (p : (a : α) -> τ a -> l) [inst': ∀ a, Inhabited (τ a)] a :
+  ⨆ (t : (α : α) -> τ α), p a (t a) = ⨆ (t : τ a), p a t := by
+    apply le_antisymm <;> simp
+    { intro i; exact le_iSup (p a) (i a) }
+    intro i
+    refine le_iSup_of_le (fun x =>
+      if h : x = a then by rw [h]; exact i else (inst' x).default) ?_
+    simp
+
+
 structure NonDet (m : Type u -> Type v) (l : Type u) (α : Type u) where
   tp  : Type u
   inh : Inhabited tp
   pre : tp -> l
   sem : tp -> m α
 
-structure NonDetCps (m : Type u -> Type v) (l : Type u) (α : Type u) where
+structure NonDetCps (m : Type u -> Type v) [Monad m] (l : Type u) [PartialOrder l] (α : Type u) where
   tpc : (α -> Type u) -> Type u
-  pre {τ : α -> Type u}              (cont : (a : α) -> τ a -> l)   : tpc τ -> l
+  pre {τ : α -> Type u} [mprop : MPropOrdered m l] (cont : (a : α) -> τ a -> l) : tpc τ -> l
   sem {τ : α -> Type u} {β : Type u} (cont : (a : α) -> τ a -> m β) : tpc τ -> m β
 
-structure NonDetT (m : Type u -> Type v) {l : Type u} [Monad m] [CompleteBooleanAlgebra l] [mprop : MPropOrdered m l] (α : Type u)
+structure NonDetT (m : Type u -> Type v) {l : Type u} [Monad m] [CompleteBooleanAlgebra l] [HasMProp m l] (α : Type u)
   extends NonDetCps m l α where
   inh (τ : α -> Type u) : (∀ a, Inhabited (τ a)) -> Inhabited (tpc τ)
-  pre_sem {τ τ' : α -> Type u} {_ : ∀ a, Inhabited (τ a)} { _ : ∀ a, Inhabited (τ' a)}
+  pre_sem_iInf [mprop : MPropOrdered m l] [MPropDetertministic m l]
+    {τ τ' : α -> Type u} {_ : ∀ a, Inhabited (τ a)} { _ : ∀ a, Inhabited (τ' a)}
     (cp₁ : (a : α) -> τ a -> l) (cp₂ : (a : α) -> τ' a -> l)
     (cs₁ : (a : α) -> τ a -> m UProp) (cs₂ : (a : α) -> τ' a -> m UProp) :
     (∀ a, ⨅ t,  cp₁ a t ⇨ MProp.μ (cs₁ a t) <= ⨅ t, cp₂ a t ⇨ MProp.μ (cs₂ a t)) ->
     ⨅ t, pre cp₁ t ⇨ MProp.μ (sem cs₁ t) <=
     ⨅ t, pre cp₂ t ⇨ MProp.μ (sem cs₂ t)
+  pre_sem_iSup  [mprop : MPropOrdered m l] [MPropDetertministic m l]
+    {τ τ' : α -> Type u} {_ : ∀ a, Inhabited (τ a)} { _ : ∀ a, Inhabited (τ' a)}
+    (cp₁ : (a : α) -> τ a -> l) (cp₂ : (a : α) -> τ' a -> l)
+    (cs₁ : (a : α) -> τ a -> m UProp) (cs₂ : (a : α) -> τ' a -> m UProp) :
+    (∀ a, ⨆ t,  cp₁ a t ⊓ MProp.μ (cs₁ a t) <= ⨆ t, cp₂ a t ⊓ MProp.μ (cs₂ a t)) ->
+    ⨆ t, pre cp₁ t ⊓ MProp.μ (sem cs₁ t) <=
+    ⨆ t, pre cp₂ t ⊓ MProp.μ (sem cs₂ t)
   sem_bind {τ : α -> Type u} {β γ} (t : tpc τ)
     (cont : (a : α) -> τ a -> m β)
     (cont' : β -> m γ) :
     sem cont t >>= cont' = sem (cont · · >>= cont') t
+  pre_mono [mprop : MPropOrdered m l] [mprop' : MPropOrdered m l] :
+    (∀ α (c : m α) post, wlp c (mprop := mprop) post = wlp c (mprop := mprop') post) ->
+    ∀ (τ : α -> Type u) (cont cont' : (a : α) -> τ a -> l),
+      (∀ x, cont x = cont' x) ->
+      pre (mprop := mprop) cont = pre (mprop := mprop') cont'
 
 @[simp]
 def NonDetT.finally (x : NonDetT m α) : NonDet m l α := {
@@ -79,11 +103,6 @@ def NonDetT.any (x : NonDetT m α) : m α := x.run x.seed
 def NonDet.validSeed (x : NonDet m l α) (pre : l) (seed : x.tp) := pre ≤ x.pre seed
 def NonDetT.validSeed (x : NonDetT m α) (pre : l) (seed : x.tp) := x.finally.validSeed pre seed
 
-@[simp]
-def NonDet.μ (x : NonDet m l UProp) : l :=  ⨅ t : x.tp, x.pre t ⇨ MProp.μ (x.sem t)
-
-def NonDetT.μ (x : NonDetT m UProp) : l := x.finally.μ
-
 variable [MPropDetertministic m l] [LawfulMonad m]
 
 def NonDetT.pure (x : α) : NonDetT m α := {
@@ -92,8 +111,10 @@ def NonDetT.pure (x : α) : NonDetT m α := {
   sem cont := cont x
 
   inh τ inh := by solve_by_elim
-  pre_sem := by introv _ _ h; simp only [h]
+  pre_sem_iInf := by introv _ _ _ h; simp only [h]
+  pre_sem_iSup := by introv _ _ _ h; simp only [h]
   sem_bind := by introv; simp
+  pre_mono := by simp; intros; solve_by_elim
 }
 
 def NonDetT.bind (x : NonDetT m α) (f : α → NonDetT m β) : NonDetT m β := {
@@ -103,11 +124,21 @@ def NonDetT.bind (x : NonDetT m α) (f : α → NonDetT m β) : NonDetT m β := 
 
   inh τ inh := by
     simp; apply x.inh; intro a; apply (f a).inh; exact inh
-  pre_sem := by
-    introv _ _ h; simp only
-    apply x.pre_sem <;> intro a <;> solve_by_elim [(f a).pre_sem, (f a).inh]
+  pre_sem_iInf := by
+    introv _ _ _ h; simp only
+    apply x.pre_sem_iInf <;> intro a <;> solve_by_elim [(f a).pre_sem_iInf, (f a).inh]
+  pre_sem_iSup := by
+    introv _ _ _ h; simp only
+    apply x.pre_sem_iSup <;> intro a <;> solve_by_elim [(f a).pre_sem_iSup, (f a).inh]
   sem_bind := by
     introv; simp [x.sem_bind, (f _).sem_bind];
+  pre_mono := by
+    simp; intros mp mp' _ τ c c' _;
+    apply x.pre_mono (mprop := mp) (τ := (fun a ↦ (f a).tpc τ)) (cont := fun a ft ↦
+      (f a).pre (mprop := mp) c ft)
+    { assumption }
+    intro a; apply (f a).pre_mono (mprop := mp) <;> assumption
+
 }
 
 def NonDetT.pick (α : Type u) [Inhabited α] : NonDetT m α := {
@@ -117,14 +148,20 @@ def NonDetT.pick (α : Type u) [Inhabited α] : NonDetT m α := {
 
   inh τ inh := by
     simp; exists default; apply (inh default).default
-  pre_sem := by
-    introv _ _; simp; rintro h ⟨a, t⟩; simp
+  pre_sem_iInf := by
+    introv _ _ _; simp; rintro h ⟨a, t⟩; simp
     apply le_trans'; apply h
     simp; intro t
     rw [<-le_himp_iff, <-le_himp_iff]
     refine iInf_le_of_le ⟨a, t⟩ ?_
     exact le_himp
+  pre_sem_iSup := by
+    introv _ _ _; simp; rintro h ⟨a, t⟩; simp
+    apply le_trans; apply h
+    simp; intro t
+    refine le_iSup_of_le ⟨a, t⟩ ?_; simp
   sem_bind := by simp
+  pre_mono := by simp; intros; ext; simp [*]
 }
 
 def NonDetT.assume  (as : Prop) : NonDetT m PUnit := {
@@ -133,11 +170,20 @@ def NonDetT.assume  (as : Prop) : NonDetT m PUnit := {
   pre cont t := ⌜as⌝ ⊓ cont .unit t
 
   inh τ inh := by solve_by_elim
-  pre_sem := by
-    introv _ _; simp only [join_himp]
+  pre_sem_iInf := by
+    introv _ _ _; simp only [join_himp]
     rw [←sup_iInf_eq, ←sup_iInf_eq];
     exact fun a ↦ sup_le_sup_left (a PUnit.unit) ⌜as⌝ᶜ
+  pre_sem_iSup := by
+    introv inh₁ inh₂ _ _; simp only [inf_assoc, <-inf_iSup_eq]
+    apply inf_le_inf_left; solve_by_elim
   sem_bind := by simp
+  pre_mono := by
+    simp; intros; ext; simp [*];
+    by_cases as = True
+    { simp_all }
+    have : as = False := by simp_all
+    simp_all
 }
 
 instance : Monad (NonDetT m) where
@@ -162,14 +208,24 @@ instance : MonadLift m (NonDetT m) where
 
     inh τ inh := by
       simp; exact ⟨fun a => inh a |>.default⟩
-    pre_sem := by
-      introv h _ _; simp only
+    pre_sem_iInf := by
+      introv h _ _ _; simp only
       simp only [μ_bind_wp (m := m), <-wlp_himp, Function.comp_apply]
       rw [<-wp_iInf, <-wp_iInf]; apply wp_cons; intro y
       rw [iInf_pi (a := y) (p := fun y iy => cp₁ y iy ⇨ MProp.μ (m := m) (cs₁ y iy))]
       rw [iInf_pi (a := y) (p := fun y iy => cp₂ y iy ⇨ MProp.μ (m := m) (cs₂ y iy))]
       solve_by_elim
+    pre_sem_iSup := by
+      introv h _ _ _; simp only
+      simp only [μ_bind_wp (m := m), wlp_join_wp, Function.comp_apply]
+      rw [<-wp_iSup, <-wp_iSup]; apply wp_cons; intro y
+      rw [iSup_pi (a := y) (p := fun y iy => cp₁ y iy ⊓ MProp.μ (m := m) (cs₁ y iy))]
+      rw [iSup_pi (a := y) (p := fun y iy => cp₂ y iy ⊓ MProp.μ (m := m) (cs₂ y iy))]
+      solve_by_elim
     sem_bind := by simp
+    pre_mono := by
+      intro _ _ wlpEq τ c c' cEq; simp; ext t
+      simp [wlpEq, cEq]
   }
 
 instance : LawfulMonad (NonDetT m) := by
@@ -178,6 +234,7 @@ instance : LawfulMonad (NonDetT m) := by
 
 section NonDetTSimplifications
 
+omit [MPropDetertministic m l]
 theorem lift_tpc {α : Type u} (x : m α) :
   (liftM (n := NonDetT m) x).tpc = ((a : α) -> · a) := rfl
 theorem lift_pre {α : Type u} τ (x : m α) :
@@ -185,8 +242,7 @@ theorem lift_pre {α : Type u} τ (x : m α) :
   fun cont t => wlp x fun a => cont a (t a) := rfl
 theorem lift_sem {α β : Type u} τ (x : m α) :
   (liftM (n := NonDetT m) x).sem (β := β) (τ := τ) = fun cont t => x >>= fun a => cont a (t a) := rfl
-
-omit [LawfulMonad m] [MPropDetertministic m l]
+omit [LawfulMonad m]
 theorem pick_tpc (τ : Type u) [Inhabited τ] :
   (pick (m := NonDetT m) τ).tpc = ((t : τ) × · t) := rfl
 theorem pick_pre (τ : Type u) τ' [Inhabited τ] :
@@ -205,6 +261,14 @@ theorem pick_sem (τ : Type u) [Inhabited τ] τ' :
 
 end NonDetTSimplifications
 
+namespace Demonic
+
+@[simp]
+def NonDet.μ (x : NonDet m l UProp) : l :=  ⨅ t : x.tp, x.pre t ⇨ MProp.μ (x.sem t)
+
+def NonDetT.μ (x : NonDetT m UProp) : l := NonDet.μ x.finally
+
+scoped
 instance : MPropOrdered (NonDetT m) l := {
   μ := NonDetT.μ
   ι := fun p => monadLift (m := m) (MProp.ι p)
@@ -220,7 +284,7 @@ instance : MPropOrdered (NonDetT m) l := {
     intros le x
     simp [liftM, monadLift, MonadLift.monadLift, bind, NonDetT.bind, NonDetT.pure]
     simp only [NonDetT.μ, NonDetT.finally]; dsimp
-    apply x.pre_sem
+    apply x.pre_sem_iInf
     { solve_by_elim }
     { intro a; solve_by_elim [(f a).inh] }
     intro a; solve_by_elim [(g a).inh]
@@ -234,8 +298,8 @@ lemma NonDetT.wp_eq (c : NonDetT m α) post :
    simp [NonDetT.μ, bind, NonDetT.bind, MProp.ι, MPropOrdered.ι]
    simp [monadLift, MonadLift.monadLift]
    simp [c.sem_bind, MProp.μ]; apply le_antisymm
-   { apply c.pre_sem <;> (try simp [iInf_const]) <;> solve_by_elim }
-   apply c.pre_sem <;> (try simp [iInf_const]) <;> solve_by_elim
+   { apply c.pre_sem_iInf <;> (try simp [iInf_const]) <;> solve_by_elim }
+   apply c.pre_sem_iInf <;> (try simp [iInf_const]) <;> solve_by_elim
 
 lemma MonadNonDet.wp_pick (τ : Type u) [Inhabited τ] (post : τ -> l) :
   wp (pick (m := NonDetT m) τ) post = ⨅ t, post t := by
@@ -251,7 +315,7 @@ lemma MonadNonDet.wp_assume as (post : PUnit -> l) :
     { apply iInf_le_of_le .unit; simp }
     simp
 
-lemma NonDetT.lift (c : m α) post :
+lemma NonDetT.wp_lift (c : m α) post :
   wp (liftM (n := NonDetT m) c) post = wp c post := by
     simp [NonDetT.wp_eq, pick_pre, wp_pure, lift_sem, lift_pre, lift_tpc]
     apply le_antisymm
@@ -265,139 +329,260 @@ lemma NonDetT.run_validSeed (x : NonDetT m α) (pre : l) (post : α -> l) (seed 
     simp [NonDetT.validSeed, triple, NonDetT.run, NonDetT.wp_eq]
     intro v h; apply le_trans'; apply h; simp [v]
 
+end Demonic
+
+namespace Angelic
+
+@[simp]
+def NonDet.μ (x : NonDet m l UProp) : l :=  ⨆ t : x.tp, x.pre t ⊓ MProp.μ (x.sem t)
+
+def NonDetT.μ (x : NonDetT m UProp) : l := NonDet.μ x.finally
+
+scoped
+instance : MPropOrdered (NonDetT m) l := {
+  μ := NonDetT.μ
+  ι := fun p => monadLift (m := m) (MProp.ι p)
+  μ_surjective := by intro p; simp [NonDetT.μ, monadLift, MonadLift.monadLift]; rw [MPropOrdered.μ_surjective]; rw [@iSup_const]
+  μ_top := by intro x; simp [NonDetT.μ, pure, NonDetT.pure, iSup_const]; apply MPropOrdered.μ_top
+  μ_bot := by intro x; simp [NonDetT.μ, pure, NonDetT.pure]; apply MPropOrdered.μ_bot
+  μ_ord_pure := by
+    intro p₁ p₂ h; simp [NonDetT.μ, pure, NonDetT.pure, iSup_const]; apply MPropOrdered.μ_ord_pure
+    assumption
+  μ_ord_bind := by
+    intro α f g
+    simp [Function.comp, Pi.hasLe, Pi.partialOrder, Pi.preorder, inferInstanceAs]
+    intros le x
+    simp [liftM, monadLift, MonadLift.monadLift, bind, NonDetT.bind, NonDetT.pure]
+    simp only [NonDetT.μ, NonDetT.finally]; dsimp
+    apply x.pre_sem_iSup
+    { solve_by_elim }
+    { intro a; solve_by_elim [(f a).inh] }
+    intro a; solve_by_elim [(g a).inh]
+  }
+
+lemma NonDetT.wp_eq (c : NonDetT m α) post :
+  wp c post =
+    ⨆ t : c.tp,
+      c.finally.pre t ⊓ wp (c.finally.sem t) post := by
+   simp [wp, liftM, monadLift, MProp.lift, MProp.μ, MPropOrdered.μ]
+   simp [NonDetT.μ, bind, NonDetT.bind, MProp.ι, MPropOrdered.ι]
+   simp [monadLift, MonadLift.monadLift]
+   simp [c.sem_bind, MProp.μ]; apply le_antisymm
+   { apply c.pre_sem_iSup <;> (try simp [iSup_const]) <;> solve_by_elim }
+   apply c.pre_sem_iSup <;> (try simp [iSup_const]) <;> solve_by_elim
+
+lemma MonadNonDet.wp_pick (τ : Type u) [Inhabited τ] (post : τ -> l) :
+  wp (pick (m := NonDetT m) τ) post = ⨆ t, post t := by
+    simp [NonDetT.wp_eq, pick_pre, pick_sem, wp_pure, pick_tpc]
+    apply le_antisymm <;> simp <;> intro i
+    { apply le_iSup_of_le i.fst; simp }
+    apply le_iSup_of_le ⟨i, .unit⟩; simp
+
+lemma MonadNonDet.wp_assume as (post : PUnit -> l) :
+  wp (assume (m := NonDetT m) as) post = ⌜as⌝ ⊓ post .unit := by
+    simp [NonDetT.wp_eq, pick_pre,wp_pure, assume_sem, assume_pre, assume_tpc]
+    apply le_antisymm
+    { exact iSup_const_le }
+    apply le_iSup_of_le .unit; simp
+
+lemma NonDetT.wp_lift (c : m α) post :
+  wp (liftM (n := NonDetT m) c) post = wp c post := by
+    simp [NonDetT.wp_eq, pick_pre, wp_pure, lift_sem, lift_pre, lift_tpc]
+    apply le_antisymm
+    { exact iSup_const_le }
+    apply le_iSup_of_le (fun _ => .unit); simp
+
+lemma NonDetT.run_validSeed (x : NonDetT m α) (pre : l) (post : α -> l) (seed : x.tp) :
+  triple pre (x.run seed) post ->
+  x.validSeed pre seed ->
+  triple pre x post := by
+    simp [NonDetT.validSeed, triple, NonDetT.run, NonDetT.wp_eq]
+    intro v h; refine le_iSup_of_le seed ?_; simp [*]
+
+end Angelic
 section ExceptT
 
 @[always_inline]
 instance (ε) [MonadExceptOf ε m] [Inhabited ε] : MonadExceptOf ε (NonDetT m) where
   throw e  := liftM (m := m) (throw e)
   /- TODO: fix me not sure how to implement it -/
-  tryCatch := fun _ c =>
+  tryCatch := fun _x c =>
     have: Inhabited (NonDetT m _) := ⟨c default⟩
     panic! "`try-catch` for nondetermenistic monad is not implemented"
 
 variable {ε : Type u}
 
-@[simp]
-def NonDetCps.toPart (c : NonDetCps (ExceptTTot ε m) l α) :
-  NonDetCps (ExceptTPart ε m) l α := {
-  tpc τ := c.tpc τ
-  pre cont := c.pre cont
-  sem cont t := (c.sem cont t).toPart }
-
-@[simp]
-private lemma himp_same_pre (x y z : l) :
-  (x ⇨ y) ⊓ (x ⇨ z) = x ⇨ y ⊓ z := by
-    simp [himp_eq, sup_inf_right]
-
-lemma wp_part_tot_aux
-  (c :  NonDetCps (ExceptTTot ε m) l α)
-  (wp_bot : noFailure m l)
-  pre_sem sem_bind inh
-  pre_sem' sem_bind' inh'
-  post :
-  let ct : NonDetT (ExceptTTot ε m) α :=
-    { c with pre_sem := pre_sem', sem_bind := sem_bind', inh := inh' }
-  let cp : NonDetT (ExceptTPart ε m) α :=
-    { c.toPart with pre_sem := pre_sem, sem_bind := sem_bind, inh := inh }
-  wp ct ⊤ ⊓ wp cp post = wp ct post := by
-    simp [NonDetT.wp_eq, NonDetT.tp, wp_part_eq_wlp (wp_bot := wp_bot)]
-    rw [← @iInf_inf_eq]; simp [wp_top_wlp]
-
-lemma NonDetT.wp_part_tot
-  (ct : NonDetT (ExceptTTot ε m) α)
-  (cp : NonDetT (ExceptTPart ε m) α)
-  (wp_bot : noFailure m l)
-  post :
-  ct.toNonDetCps = cp.toNonDetCps ->
-  wp ct ⊤ ⊓ wp cp post = wp ct post := by
-    rcases ct with ⟨ct⟩; rcases cp with ⟨cp⟩
-    rintro rfl; apply wp_part_tot_aux (wp_bot := wp_bot)
-
 
 end ExceptT
 
+def ite.fst {α β} {p : Prop} [Decidable p] (x : if p then α else β) (h : p) : α := by
+  rw [if_pos h] at x; exact x
+
+
+def ite.snd {α β} {p : Prop} [Decidable p] (x : if p then α else β) (h : ¬p) : β := by
+  rw [if_neg h] at x; exact x
+
+def bite.fst {α β: Type u} {p : Prop} [instD : Decidable p] : (x : bif p then α else β) -> (h : p) -> α := by
+  rcases instD with (h|h) <;> dsimp [decide]
+  { exact fun _ f => by contradiction  }
+  exact fun x _ => x
+def bite.snd {α β : Type u} {p : Prop} [instD : Decidable p] : (x : bif p then α else β) -> (h : ¬p) -> β := by
+  rcases instD with (h|h) <;> dsimp [decide]
+  { exact fun x _ => x }
+  exact fun _ f => by contradiction
+
+
+
+private lemma iInf_bif_pos {α β : Type u} (cnd : Prop) [instD : Decidable cnd] (h : cnd)
+  (f : α -> l) : ⨅ x : bif cnd then α else β, f (bite.fst x h) = ⨅ x : α, f x := by
+  apply le_antisymm
+  { simp; intro i; apply iInf_le_of_le (by simp_all; assumption);
+    cases instD <;> simp [bite.fst]; contradiction }
+  simp; intro i; apply iInf_le_of_le (by simp [h] at i; assumption)
+  cases instD <;> simp [bite.fst]; contradiction
+
+private lemma iInf_bif_neg {α β : Type u} (cnd : Prop) [instD : Decidable cnd] (h : ¬cnd)
+  (f : β -> l) : ⨅ x : bif cnd then α else β, f (bite.snd x h) = ⨅ x : β, f x := by
+  apply le_antisymm
+  { simp; intro i; apply iInf_le_of_le (by simp_all; assumption)
+    cases instD <;> simp [bite.snd]; contradiction }
+  simp; intro i; apply iInf_le_of_le (by simp [h] at i; assumption);
+  cases instD <;> simp [bite.snd]; contradiction
+
+private lemma iSup_bif_neg {α β : Type u} (cnd : Prop) [instD : Decidable cnd] (h : ¬cnd)
+  (f : β -> l) : ⨆ x : bif cnd then α else β, f (bite.snd x h) = ⨆ x : β, f x := by
+  apply le_antisymm
+  { simp; intro i; apply le_iSup_of_le (by simp [h] at i; assumption);
+    cases instD <;> simp [bite.snd]; contradiction }
+  simp; intro i; apply le_iSup_of_le (by simp_all; assumption);
+  cases instD <;> simp [bite.snd]; contradiction
+
+private lemma iSup_bif_pos {α β : Type u} (cnd : Prop) [instD : Decidable cnd] (h : cnd)
+  (f : α -> l) : ⨆ x : bif cnd then α else β, f (bite.fst x h) = ⨆ x : α, f x := by
+  apply le_antisymm
+  { simp; intro i; apply le_iSup_of_le (by simp [h] at i; assumption);
+    cases instD <;> simp [bite.fst]; contradiction  }
+  simp; intro i; apply le_iSup_of_le  (by simp_all; assumption)
+  cases instD <;> simp [bite.fst]; contradiction
+
+def NonDetT.ite {α : Type u} (cnd : Prop) [instD : Decidable cnd] (thn : NonDetT m α) (els : NonDetT m α) : NonDetT m α := {
+  tpc τ := bif cnd then thn.tpc τ else els.tpc τ
+  pre {τ} _ cont t := if h : cnd then thn.pre cont (bite.fst t h) else els.pre cont (bite.snd t h)
+  sem {τ β} cont t := if h : cnd then thn.sem cont (bite.fst t h) else els.sem cont (bite.snd t h)
+
+  inh τ inh := by
+    simp; cases (decide cnd) <;> simp <;> solve_by_elim [thn.inh, els.inh]
+  pre_sem_iInf := by
+    dsimp; split_ifs with h <;> introv <;> intros
+    { repeat rw [iInf_bif_pos (instD := instD) (f := fun t => thn.pre _ t ⇨ MPropOrdered.μ (thn.sem _ t))]
+      apply thn.pre_sem_iInf <;> assumption }
+    repeat rw [iInf_bif_neg (instD := instD) (f := fun t => els.pre _ t ⇨ MPropOrdered.μ (els.sem _ t))]
+    apply els.pre_sem_iInf <;> assumption
+  pre_sem_iSup := by
+    dsimp; split_ifs with h <;> introv <;> intros
+    { repeat rw [iSup_bif_pos (instD := instD) (f := fun t => thn.pre _ t ⊓ MPropOrdered.μ (thn.sem _ t))]
+      apply thn.pre_sem_iSup <;> assumption }
+    repeat rw [iSup_bif_neg (instD := instD) (f := fun t => els.pre _ t ⊓ MPropOrdered.μ (els.sem _ t))]
+    apply els.pre_sem_iSup <;> assumption
+  sem_bind     := by
+    simp; split_ifs <;> intros <;> solve_by_elim [thn.sem_bind, els.sem_bind]
+  pre_mono     := by
+    simp; split_ifs <;> intros
+    { ext; rw [@thn.pre_mono] <;> try simp [*] }
+    ext; rw [@els.pre_mono] <;> try simp [*]
+}
+
+omit [MPropDetertministic m l] [LawfulMonad m] in
+@[simp↑ high]
+lemma NonDetT.ite_eq {α : Type u} (x : NonDetT m α) (y : NonDetT m α) (cond : Prop) [dec : Decidable cond] :
+  (if cond then x else y) = NonDetT.ite cond x y := by
+    split_ifs with h
+    { have : cond = True := by simp_all
+      cases this;
+      simp [ite, decide]
+      cases dec <;> simp_all
+      rcases x with ⟨⟨⟩⟩; simp [bite.fst] }
+    have : cond = False := by simp_all
+    cases this;
+    simp [ite, decide]
+    cases dec <;> simp_all
+    rcases y with ⟨⟨⟩⟩; simp [bite.snd]
+    contradiction
+section
+open Demonic
+
+private lemma meet_himp (x x' y z : l) :
+  x = x' ->
+  (x ⇨ y) ⊓ (x' ⇨ z) = x ⇨ (y ⊓ z) := by
+  rintro rfl
+  simp [himp_eq]; rw [@sup_inf_right]
+
+private lemma le_coml_sup (x y z : l) :
+  y <= x ⊔ z -> xᶜ <= yᶜ ⊔ z := by
+  intro h;
+  rw [sup_comm, <-himp_eq]; simp
+  rw [inf_comm, <-le_himp_iff, himp_eq]; simp
+  rwa [sup_comm]
+
+
+lemma NonDetT.wp_tot_part ε (c : NonDetT (ExceptT ε m) α) post :
+  [totl| wp c ⊤] ⊓ [part| wp c post] = [totl| wp c post] := by
+  open PartialCorrectness in rw [@NonDetT.wp_eq]
+  open TotalCorrectness in repeat rw [@NonDetT.wp_eq]
+  unfold NonDetT.tp
+  simp [<-iInf_inf_eq, meet_himp]
+  open TotalCorrectness in
+  conv =>
+    enter [1,1]; ext; rw [meet_himp]; rfl
+    erw [@c.pre_mono (cont := ⊤) (τ := fun _ => PUnit)]; rfl
+    tactic =>
+      introv; simp [wlp, wp_part_eq, wp_tot_eq]
+      apply le_antisymm <;> simp
+      { constructor
+        { apply le_coml_sup; rw [<-wp_or]; apply wp_cons
+          rintro (_|_) <;> simp }
+        refine le_sup_of_le_right ?_; apply wp_cons
+        rintro (_|_) <;> simp }
+      constructor
+      { apply le_coml_sup; rw [<-wp_or]; apply wp_cons
+        rintro (_|_) <;> simp }
+      rw [sup_comm, <-himp_eq]; simp [<-wp_and]
+      apply wp_cons; rintro (_|_) <;> simp
+    tactic => simp
+  simp [_root_.wp_tot_part]
+
+set_option quotPrecheck false in
+notation "[totl😇|" t "]" => open TotalCorrectness Angelic in t
+set_option quotPrecheck false in
+notation "[part😈|" t "]" => open PartialCorrectness Demonic in t
+
+lemma NonDetT.iwp_part_wp_tot_eq ε (c : NonDetT (ExceptT ε m) α) post
+  (wp_bot : ∀ α (c : m α), wp c ⊥ = ⊥)
+  (wp_top : ∀ α (c : m α), wp c ⊤ = ⊤) :
+  [part😈| iwp c post] = [totl😇| wp c post] := by
+    simp [iwp, NonDetT.wp_eq, Angelic.NonDetT.wp_eq, compl_iInf, -compl_himp, himp_eq]
+    simp (disch := assumption) [wp_tot_eq_iwp_part]
+    simp [inf_comm]; congr; ext; congr 1
+    erw [@c.pre_mono (τ := fun _ => PUnit)] <;> try simp
+    introv; simp [wlp, wp_part_eq, wp_tot_eq]
+    apply le_antisymm <;> simp
+    { constructor
+      { apply le_coml_sup; rw [<-wp_or]; apply wp_cons
+        rintro (_|_) <;> simp }
+      rw [sup_comm, <-himp_eq]; simp [<-wp_and]
+      apply wp_cons; rintro (_|_) <;> simp }
+    constructor
+    { apply le_coml_sup; rw [<-wp_or]; apply wp_cons
+      rintro (_|_) <;> simp }
+    refine le_sup_of_le_right ?_; apply wp_cons
+    rintro (_|_) <;> simp
+
+
+
+
+
+
+end
+
+
 end NonDetermenisticTransformer
-
-section Example
-
-
-abbrev myM := NonDetT (StateT Nat (ExceptTTot String Id))
-
-def ex : myM Unit :=
-  do
-    set 0
-    let x <- get
-    assume (x < 1)
-    throw "e"
-
-
-example (P : _ -> Prop) : P (ex.finally) := by
-  dsimp [ex, bind, pure, NonDetT.finally]
-  unfold NonDetT.bind;
-  simp [set, get, getThe, MonadStateOf.get]
-  simp [pick_tpc,
-        assume_tpc,
-        lift_tpc,
-        assume_pre,
-        lift_pre,
-        lift_sem,
-        assume_sem,
-        -bind_pure_comp,
-        Id
-        ]
-  sorry
-
-def ex' : myM Unit :=
-  do
-    let x <- pick ℕ
-    let y <- pick ℕ
-    assume (x < y)
-    set (y - x)
-
-example (P : _ -> Prop) : P (ex'.finally) := by
-  dsimp [ex', bind, pure, NonDetT.finally]
-  unfold NonDetT.bind;
-  simp [set, get, getThe, MonadStateOf.get]
-  simp only [pick_tpc,
-        assume_tpc,
-        lift_tpc,
-        assume_pre,
-        lift_pre,
-        lift_sem,
-        pick_pre,
-        pick_sem,
-        assume_sem,
-        wp_pure,
-        Id
-        ]
-  sorry
-
-
-def ex'' : myM Unit :=
-  do
-    let x <- pick ℕ
-    assume (x < 1)
-    let s <- get
-    let y <- pick ℕ
-    assume (y < s)
-    set (y - x)
-
-example (P : _ -> Prop) : P (ex''.finally) := by
-  dsimp [ex'', bind, pure, NonDetT.finally]
-  unfold NonDetT.bind;
-  simp [set, get, getThe, MonadStateOf.get]
-  simp [pick_tpc,
-        assume_tpc,
-        lift_tpc,
-        assume_pre,
-        lift_pre,
-        lift_sem,
-        pick_sem,
-        pick_pre,
-        wp_pure,
-        assume_sem,
-        Id
-        ]
-  sorry
-
-end Example
